Progress on Classifiers

Capless/Classifier.lean
@@ -348,28 +348,119 @@ inductive Intersect : Kind -> Kind -> Kind -> Prop where
   | singleton_r : r2.Subclass r1 -> Intersect (.node r1 ex1) (.node r2 ex2) (.node r2 (ex1 ++ ex2))
   | singleton_disj : r1.Disjoint r2 -> Intersect (.node r1 ex1) (.node r2 ex2) .empty
 
-inductive Kind.Subkind : Kind -> Kind -> Prop where
-  | empty_l : Subkind .empty K
-  | union_l : Subkind K1 K -> Subkind K2 K -> Subkind (.union K1 K2) K
-  | absurd_l : ContainsSupOf ex1 r1 -> Subkind (.node r1 ex1) K
+inductive Kind.Subtract : Kind -> Kind -> Kind -> Prop where
+  | empty_l : Subtract .empty K .empty
+  | union_l : Subtract K1 K R1 -> Subtract K2 K R2 -> Subtract (.union K1 K2) K (.union R1 R2)
+  | absurd_l : ContainsSupOf ex1 r1 -> Subtract (.node r1 ex1) K .empty
   | excl_subclass_r :
-    a.StrictSub r2 -> -- not absurd
+    a.StrictSub r2 ->
     ContainsSupOf ex1 a ->
-    Subkind (.node r1 ex1) (.node r2 ex2) ->
-    Subkind (.node r1 ex1) (.node r2 (a :: ex2))
+    Subtract (.node r1 ex1) (.node r2 ex2) R ->
+    Subtract (.node r1 ex1) (.node r2 (a :: ex2)) R
   | excl_disjoint_r :
-    a.StrictSub r2 -> -- not absurd
+    a.StrictSub r2 ->
     a.Disjoint r1 ->
-    Subkind (.node r1 ex1) (.node r2 ex2) ->
-    Subkind (.node r1 ex1) (.node r2 (a :: ex2))
+    Subtract (.node r1 ex1) (.node r2 ex2) R ->
+    Subtract (.node r1 ex1) (.node r2 (a :: ex2)) R
   | excl_irrelevant_r :
     a.Disjoint r2 ->
-    Subkind (.node r1 ex1) (.node r2 ex2) ->
-    Subkind (.node r1 ex1) (.node r2 (a :: ex2))
+    Subtract (.node r1 ex1) (.node r2 ex2) R ->
+    Subtract (.node r1 ex1) (.node r2 (a :: ex2)) R
+  | excl_r :
+    a.Disjoint r2 ->
+    a.Subclass r1 ->
+    Subtract (.node r1 ex1) (.node r2 ex2) R ->
+    Subtract (.node r1 ex1) (.node r2 (a :: ex2)) (.union R (.node a ex1))
+  | subclass_l :
+    r2.Subclass r1 ->
+    Subtract (.node r1 ex1) (.node r2 []) (.node r1 (r2 :: ex1))
   | subclass_r :
     r1.Subclass r2 ->
-    Subkind (.node r1 ex1) (.node r2 [])
-  -- | union_r : Intersect K K1 R -> Subkind R K2 -> Subkind K (.union K1 K2) -- wrong. needs subtract
+    Subtract (.node r1 ex1) (.node r2 []) .empty
+  | irrelevant_r :
+    r1.Disjoint r2 ->
+    Subtract (.node r1 ex1) (.node r2 []) (.node r1 ex1)
+  | union_r :
+    Subtract (.node r1 ex1) K1 R1 ->
+    Subtract R1 K2 R2 ->
+    Subtract (.node r1 ex1) (.union K1 K2) R2
+
+inductive Kind.Subkind : Kind -> Kind -> Prop where
+  | subtract : Subtract K1 K2 R -> IsEmpty R -> Subkind K1 K2
+
+theorem Kind.Subtract.from_empty (hs : Subtract K1 K2 R) (he : IsEmpty K1) : IsEmpty R := by
+  induction hs
+  case empty_l => constructor
+  case union_l ih1 ih2 =>
+    cases he with
+    | union he1 he2 => exact .union (ih1 he1) (ih2 he2)
+  case absurd_l => constructor
+  case excl_subclass_r ih => exact ih he
+  case excl_disjoint_r ih => exact ih he
+  case excl_irrelevant_r ih => exact ih he
+  case excl_r _ hsub _ ih =>
+    cases he with
+    | absurd ha => exact .union (ih (.absurd ha)) (.absurd (ha.trans_subclass hsub))
+  case subclass_l hsub =>
+    cases he with
+    | absurd ha => apply! IsEmpty.absurd $ .there _
+  case subclass_r => constructor
+  case irrelevant_r =>
+    cases he with
+    | absurd ha => exact .absurd ha
+  case union_r ih1 ih2 =>
+    cases he with
+    | absurd ha => exact ih2 (ih1 (.absurd ha))
+
+theorem Kind.Subtract.empty_r_inv (hs : Subtract K1 K2 R) (he : IsEmpty R) (hek2 : IsEmpty K2) : IsEmpty K1 := by
+  induction hs
+  case empty_l => constructor
+  case union_l ih1 ih2 =>
+    cases he with
+    | union he1 he2 => exact .union (ih1 he1 hek2) (ih2 he2 hek2)
+  case absurd_l ha => exact .absurd ha
+  case excl_subclass_r hss hc _ ih =>
+    cases hek2 with
+    | absurd ha =>
+      cases ha
+      case here hsub => exact (hss.antisymm hsub).elim
+      case there ha => exact ih he (.absurd ha)
+  case excl_disjoint_r hss _ _ ih =>
+    cases hek2 with
+    | absurd ha =>
+      cases ha
+      case here hsub => exact (hss.antisymm hsub).elim
+      case there ha => exact ih he (.absurd ha)
+  case excl_irrelevant_r hd _ ih =>
+    cases hek2 with
+    | absurd ha =>
+      cases ha
+      case here hsub => exact (hd.symm.not_subclass hsub).elim
+      case there ha => exact ih he (.absurd ha)
+  case excl_r hd hsub _ ih =>
+    cases he with
+    | union heR heA =>
+      cases hek2 with
+      | absurd ha =>
+        cases ha
+        case here hsub2 => exact (hd.symm.not_subclass hsub2).elim
+        case there ha => exact ih heR (.absurd ha)
+  case subclass_l =>
+    cases hek2 with
+    | absurd ha => cases ha
+  case subclass_r =>
+    cases hek2 with
+    | absurd ha => cases ha
+  case irrelevant_r =>
+    cases hek2 with
+    | absurd ha => cases ha
+  case union_r ih1 ih2 =>
+    cases hek2 with
+    | union he2a he2b => exact ih1 (ih2 he he2b) he2a
+
+theorem Kind.Subkind.empty_r_inv (hs : Subkind K1 K2) (he : IsEmpty K2) : IsEmpty K1 := by
+  cases hs
+  apply! Subtract.empty_r_inv
 
 inductive Kind.Disjoint : Kind -> Kind -> Prop where
   | empty_l: Disjoint .empty K
@@ -519,56 +610,335 @@ theorem Kind.Disjoint.absurd_l' (hs : ContainsSupOf ex1 r1) : Disjoint (.node r1
   case node => apply! absurd_l
   case union ha hb => apply! union_r
 
-theorem Kind.Subkind.empty_r_inv (hs : Subkind K1 K2) (he : IsEmpty K2) : IsEmpty K1 := by
+theorem Kind.Disjoint.refine_subtract_l (hd : Disjoint K1 K) (hs : Subtract K1 K2 R) : Disjoint R K := by
   induction hs
-  case empty_l => constructor
-  case union_l ha hb => apply! IsEmpty.union (ha _) (hb _)
-  case absurd_l => apply! IsEmpty.absurd
-  case excl_subclass_r hss hc hs ih =>
-    cases he
-    rename_i he
-    cases he
-    case here he => cases hss.antisymm he
-    case there he => apply! ih (.absurd _)
-  case excl_disjoint_r hss _ _ ih =>
-    cases he
-    rename_i he
-    cases he
-    case here he => cases hss.antisymm he
-    case there he => apply! ih (.absurd _)
-  case excl_irrelevant_r hd hs ih =>
-    cases he
-    rename_i he
-    cases he
-    case here he => cases hd.symm.not_subclass he
-    case there he => apply! ih (.absurd _)
-  case subclass_r => cases he; rename_i he; cases he
-  case union_r hi hs ih =>
-    cases he
-
-
-
-
-theorem Kind.Disjoint.refine_subkind_l' (hd : K1.Disjoint (.node r2 ex2)) (hs : Subkind L K1) : L.Disjoint (.node r2 ex2) := by
-  induction hs with
-  | empty_l => exact .empty_l
-  | union_l _ _ ih1 ih2 => exact .union_l (ih1 hd) (ih2 hd)
-  | absurd_l ha =>
-    apply absurd_l' ha
-  | excl_subclass_r hss hc hs ih =>
-    cases hd
-    case absurd_l hc =>
-      cases hc
-      case here hc => cases hss.antisymm hc
-      case there hc =>
-
-
-  | excl_disjoint_r _ _ _ ih => exact ih (hd.excl_cons_l)
-  | excl_irrelevant_r _ _ ih => exact ih (hd.excl_cons_l)
-  | subclass_r hsub => exact hd.refine_subclass_node hsub
-  | @union_r K K1' R K2' hi hs' ih =>
+  case empty_l => exact .empty_l
+  case union_l ih1 ih2 =>
     have ⟨hd1, hd2⟩ := hd.union_l_inv
-    exact refine_union_r hi hs' hd1 hd2 ih
+    exact .union_l (ih1 hd1) (ih2 hd2)
+  case absurd_l => exact .empty_l
+  case excl_subclass_r ih => exact ih hd
+  case excl_disjoint_r ih => exact ih hd
+  case excl_irrelevant_r ih => exact ih hd
+  case excl_r _ hsub _ ih => exact .union_l (ih hd) (hd.refine_subroot_l hsub)
+  case subclass_l hsub => apply! append_excl_l (ex1:=[_])
+  case subclass_r => exact .empty_l
+  case irrelevant_r => exact hd
+  case union_r ih1 ih2 => exact ih2 (ih1 hd)
+
+theorem Kind.Subtract.empty_or_subroot (hs : Subtract (.node r1 ex1) (.node r2 ex2) R) (he : IsEmpty R) : ContainsSupOf ex1 r1 ∨ r1.Subclass r2 := by
+  cases hs
+  case absurd_l => left; assumption
+  case excl_subclass_r hss hsc hs =>
+    cases hs.empty_or_subroot he <;> aesop
+  case excl_disjoint_r hss hsc hs =>
+    cases hs.empty_or_subroot he <;> aesop
+  case excl_irrelevant_r hd hs =>
+    cases hs.empty_or_subroot he <;> aesop
+  case excl_r hs =>
+    cases he
+    rename_i he1 he2
+    cases hs.empty_or_subroot he1 <;> aesop
+  case subclass_l hs =>
+    cases he
+    rename_i he
+    cases he
+    case here he => cases hs.antisymm he; right; constructor
+    case there => aesop
+  case subclass_r => aesop
+  case irrelevant_r => cases he; aesop
+
+-- theorem Kind.Disjoint.refine_subclass_l (hd : Disjoint (.node r2 ex2) K) (hs : Classifier.Subclass r1 r2) : ContainsSupOf ex2 r2 ∨ Disjoint (.node r1 ex1) K := by
+--   cases hd
+--   case empty_r => right; apply! empty_r
+--   case union_r h1 h2 =>
+--     cases h1.refine_subclass_l hs (ex1:=ex1); aesop
+--     cases h2.refine_subclass_l hs (ex1:=ex1); aesop
+--     right; apply! union_r
+--   case absurd_l hsc => aesop
+--   case absurd_r hsc => right; apply! absurd_r
+--   case root hd => right; apply root $ hd.refines_subclass_l hs
+--   case excl_l hsc => right; apply excl_l $ hsc.trans_subclass hs
+--   case excl_r r2' ex2' hsc =>
+--     induction hsc
+--     case here a xs r2' hss =>
+--       cases Classifier.subclass_or_disjoint a r1
+--       case inl hs1 =>
+
+theorem Kind.Disjoint.refine_disjoint_subtract_l (hd2 : Disjoint K2 K) (hs : Subtract K1 K2 R) (hdr : Disjoint R K) : Disjoint K1 K := by
+  induction hs generalizing K
+  case empty_l => apply empty_l
+  case union_l ih1 ih2 =>
+    have ⟨_, _⟩ := hdr.union_l_inv
+    apply! union_l (ih1 _ _) (ih2 _ _)
+  case absurd_l => apply! absurd_l'
+  case excl_subclass_r ex1 a r1 r2 ex2 _  hss hsc hs ih =>
+    generalize h : node r2 (a :: ex2) = L at hd2
+    induction hd2 generalizing K2 <;> try cases h
+    case empty_r => apply! empty_r
+    case union_r ha hb =>
+      simp_all
+      have ⟨_, _⟩ := hdr.union_r_inv
+      apply! union_r (ha _) (hb _)
+    case absurd_l hsc =>
+      cases hsc
+      case here hsc => cases hss.antisymm hsc
+      case there hsc =>
+        apply ih _ hdr
+        apply! absurd_l
+    case absurd_r => apply! absurd_r
+    case root hd1 => apply ih (.root hd1) hdr
+    case excl_l hsc => apply! ih (.excl_l _)
+    case excl_r hsc =>
+      cases hsc
+      case here hs => apply excl_r $ hsc.trans_subclass hs
+      case there hsc => apply! ih (excl_r _)
+  case excl_disjoint_r r1 ex1 r2 ex2 _ a hss hd hs ih =>
+    generalize h : node r2 (a :: ex2) = L at hd2
+    induction hd2 generalizing K2 <;> try cases h
+    case empty_r => apply! empty_r
+    case union_r ha hb =>
+      simp_all
+      have ⟨_, _⟩ := hdr.union_r_inv
+      apply! union_r (ha _) (hb _)
+    case absurd_l hsc =>
+      cases hsc
+      case here hsc => cases hss.antisymm hsc
+      case there hsc =>
+        apply ih _ hdr
+        apply! absurd_l
+    case absurd_r => apply! absurd_r
+    case root hd1 => apply ih (.root hd1) hdr
+    case excl_l hsc => apply! ih (.excl_l _)
+    case excl_r hsc =>
+      cases hsc
+      case here hs => apply! root $ hd.symm.refines_subclass_r _
+      case there hsc => apply! ih (excl_r _)
+  case excl_irrelevant_r r1 ex1 r2 ex2 _ a hd hs ih =>
+    generalize h : node r2 (a :: ex2) = L at hd2
+    induction hd2 generalizing K2 <;> try cases h
+    case empty_r => apply! empty_r
+    case union_r ha hb =>
+      simp_all
+      have ⟨_, _⟩ := hdr.union_r_inv
+      apply! union_r (ha _) (hb _)
+    case absurd_l hsc =>
+      cases hsc
+      case here hsc => cases hd.symm.not_subclass hsc
+      case there hsc =>
+        apply ih _ hdr
+        apply! absurd_l
+    case absurd_r => apply! absurd_r
+    case root hd1 => apply ih (.root hd1) hdr
+    case excl_l hsc => apply! ih (.excl_l _)
+    case excl_r hsc =>
+      cases hsc
+      case here hs => apply ih _ hdr; apply root; apply! hd.symm.refines_subclass_r
+      case there hsc => apply! ih (excl_r _)
+  case excl_r r1 ex1 r2 ex2 _ a hd hsc hs ih =>
+    have ⟨hdr', hd'⟩ := hdr.union_l_inv
+    generalize h : node r2 (a :: ex2) = L at hd2
+    induction hd2 generalizing K2 <;> try cases h
+    case empty_r => apply! empty_r
+    case union_r ha hb =>
+      simp_all
+      have ⟨_, _⟩ := hdr.union_r_inv
+      have ⟨_, _⟩ := hdr'.union_r_inv
+      have ⟨hl, hr⟩ := hd'.union_r_inv
+      apply! union_r (ha _ _ _) (hb _ _ _)
+    case absurd_l hsc =>
+      cases hsc
+      case here hsc => cases hd.symm.not_subclass hsc
+      case there hsc =>
+        apply ih _ hdr'
+        apply! absurd_l
+    case absurd_r => apply! absurd_r
+    case root hd1 => apply ih (.root hd1) hdr'
+    case excl_l hsc => apply! ih (.excl_l _)
+    case excl_r hsc =>
+      cases hsc
+      case here hs =>
+
+        --  apply! root $ hd.symm.refines_subclass_r _
+      case there hsc => apply! ih (excl_r _)
+
+
+
+
+
+-- theorem Kind.Disjoint.refine_subkind_l' (hd : Disjoint K2 K) (hs : Subtract K1 K2 R) (he : IsEmpty R) : Disjoint K1 K := by
+--   induction hs generalizing K
+--   case empty_l => exact .empty_l
+--   case union_l ih1 ih2 =>
+--     cases he with
+--     | union he1 he2 => exact .union_l (ih1 hd he1) (ih2 hd he2)
+--   case absurd_l hc => exact absurd_l' hc
+--   case excl_subclass_r ex1 a r1 r2 ex2 _ hss hsc hs ih =>
+--     generalize h : node r2 (a :: ex2) = L at hd
+--     induction hd generalizing K2 <;> try cases h
+--     case empty_r => apply! empty_r
+--     case union_r ha hb => subst_vars; simp_all; apply! union_r ha hb
+--     case absurd_l hsc =>
+--       cases hsc
+--       case here hsc => cases hss.antisymm hsc
+--       case there hsc =>
+--         cases hs.empty_r_inv he (.absurd hsc)
+--         apply! absurd_l
+--     case absurd_r => apply! absurd_r
+--     case root hd =>
+--       cases hs.empty_or_subroot he
+--       case inl hsc => apply! absurd_l
+--       case inr hss => apply root $ hd.refines_subclass_l hss
+--     case excl_l hsc =>
+--       cases hs.empty_or_subroot he
+--       case inl hsc => apply! absurd_l
+--       case inr hss => apply! excl_l $ hsc.trans_subclass hss
+--     case excl_r hsc1 =>
+--       cases hsc1
+--       case here hsc1 => apply excl_r $ hsc.trans_subclass hsc1
+--       case there hsc1 => apply ih _ he; apply! excl_r
+--   case excl_disjoint_r r1 ex1 r2 ex2 _ a hss hd hs ih =>
+--     simp_all
+--     generalize h : node r2 (a :: ex2) = L at hd
+--     induction hd generalizing K2 <;> try cases h
+--     case empty_r => apply! empty_r
+--     case union_r ha hb => subst_vars; simp_all; apply! union_r ha hb
+--     case absurd_l hsc =>
+--       cases hsc
+--       case here hsc => cases hss.antisymm hsc
+--       case there hsc =>
+--         cases hs.empty_r_inv he (.absurd hsc)
+--         apply! absurd_l
+--     case absurd_r => apply! absurd_r
+--     case root hd =>
+--       cases hs.empty_or_subroot he
+--       case inl hsc => apply! absurd_l
+--       case inr hss => apply root $ hd.refines_subclass_l hss
+--     case excl_l hsc =>
+--       cases hs.empty_or_subroot he
+--       case inl hsc => apply! absurd_l
+--       case inr hss => apply! excl_l $ hsc.trans_subclass hss
+--     case excl_r hsc1 =>
+--       cases hsc1
+--       case here hsc1 => apply root $ (hd.refines_subclass_l hsc1).symm
+--       case there hsc1 => apply ih _; apply! excl_r
+--   case excl_irrelevant_r r1 ex1 r2 ex2 _ a hd1 hs ih =>
+--     simp_all
+--     generalize h : node r2 (a :: ex2) = L at hd
+--     induction hd generalizing K2 <;> try cases h
+--     case empty_r => apply! empty_r
+--     case union_r ha hb => subst_vars; simp_all; apply! union_r ha hb
+--     case absurd_l hsc =>
+--       cases hsc
+--       case here hsc => cases hd1.symm.not_subclass hsc
+--       case there hsc =>
+--         cases hs.empty_r_inv he (.absurd hsc)
+--         apply! absurd_l
+--     case absurd_r => apply! absurd_r
+--     case root hd =>
+--       cases hs.empty_or_subroot he
+--       case inl hsc => apply! absurd_l
+--       case inr hss => apply root $ hd.refines_subclass_l hss
+--     case excl_l hsc =>
+--       cases hs.empty_or_subroot he
+--       case inl hsc => apply! absurd_l
+--       case inr hss => apply! excl_l $ hsc.trans_subclass hss
+--     case excl_r hsc1 =>
+--       cases hsc1
+--       case here hsc1 => apply ih; apply root; apply hd1.symm.refines_subclass_r hsc1
+--       case there hsc1 => apply ih _; apply! excl_r
+--   case excl_r r1 ex1 r2 ex2 _ a hd1 hsc hs ih =>
+--     cases he
+--     rename_i he he1
+--     cases he1
+--     simp_all
+--     rename_i he1
+--     generalize h : node r2 (a :: ex2) = L at hd
+--     induction hd generalizing K2 <;> try cases h
+--     case empty_r.refl => apply! empty_r
+--     case union_r.refl ha hb => subst_vars; simp_all; apply! union_r ha hb
+--     case absurd_l.refl hsc =>
+--       cases hsc
+--       case here hsc => cases hd1.symm.not_subclass hsc
+--       case there hsc =>
+--         cases hs.empty_r_inv he (.absurd hsc)
+--         apply! absurd_l
+--     case absurd_r.refl => apply! absurd_r
+--     case root.refl hd =>
+--       cases hs.empty_or_subroot he
+--       case inl hsc => apply! absurd_l
+--       case inr hss => apply root $ hd.refines_subclass_l hss
+--     case excl_l.refl hsc =>
+--       cases hs.empty_or_subroot he
+--       case inl hsc => apply! absurd_l
+--       case inr hss => apply! excl_l $ hsc.trans_subclass hss
+--     case excl_r.refl hsc1 =>
+--       cases hsc1
+--       case here hsc1 => apply ih; apply root; apply hd1.symm.refines_subclass_r hsc1
+--       case there hsc1 => apply ih _; apply! excl_r
+--   case subclass_l r1 ex1 r2 hs =>
+--     cases he
+--     rename_i he
+--     cases he
+--     case here he => cases hs.antisymm he; have h := hd.append_excl_l (ex1:=ex1); simp at h; assumption
+--     case there => apply! absurd_l'
+--   case subclass_r r1 ex1 r2 hs =>
+--     generalize h : node r2 [] = L at hd
+--     induction hd <;> try cases h
+--     case empty_r => apply! empty_r
+--     case union_r ha hb => simp_all; apply! union_r
+--     case absurd_l hsc => cases hsc
+--     case absurd_r => apply! absurd_r
+--     case root hd => apply! root $ hd.refines_subclass_l _
+--     case excl_l hsc => apply! excl_l $ hsc.trans_subclass _
+--     case excl_r hsc => cases hsc
+--   case irrelevant_r hd =>
+--     cases he
+--     apply! absurd_l'
+--   case union_r ha hb =>
+
+    -- have ⟨hl, hr⟩ := hd.union_l_inv
+    -- simp_all
+    -- apply ha hl
+
+
+
+
+
+
+
+
+
+
+
+
+
+
+
+
+
+
+
+-- theorem Kind.Disjoint.refine_subkind_l' (hd : K1.Disjoint (.node r2 ex2)) (hs : Subkind L K1) : L.Disjoint (.node r2 ex2) := by
+--   induction hs with
+--   | empty_l => exact .empty_l
+--   | union_l _ _ ih1 ih2 => exact .union_l (ih1 hd) (ih2 hd)
+--   | absurd_l ha =>
+--     apply absurd_l' ha
+--   | excl_subclass_r hss hc hs ih =>
+--     cases hd
+--     case absurd_l hc =>
+--       cases hc
+--       case here hc => cases hss.antisymm hc
+--       case there hc =>
+
+
+--   | excl_disjoint_r _ _ _ ih => exact ih (hd.excl_cons_l)
+--   | excl_irrelevant_r _ _ ih => exact ih (hd.excl_cons_l)
+--   | subclass_r hsub => exact hd.refine_subclass_node hsub
+--   | @union_r K K1' R K2' hi hs' ih =>
+--     have ⟨hd1, hd2⟩ := hd.union_l_inv
+--     exact refine_union_r hi hs' hd1 hd2 ih
 
 -- theorem Kind.Disjoint.excl_cons_l (hd : Disjoint (.node r1 (a :: ex1)) K2) : Disjoint (.node r1 ex1) K2 := by
 --   cases hd with
